Started new proof of insert_is_redblack_checker_correct
... but too much abstraction getting in the way of brute force :)

src/GenHigh.v
@@ -146,6 +146,19 @@ Hypothesis semElementsSize:
   forall {A} (l: list A) (def : A) s,
     (semGenSize (elements def l) s) <--> if l is nil then [set def] else l.
 
+Definition genPair {A B : Type} (ga : G A) (gb : G B) : G (A * B) :=
+  liftGen2 pair ga gb.
+
+Definition curry {A B C : Type} (f : A -> B -> C) (ab : A * B) :=
+  match ab with
+  | (a,b) => f a b
+  end.
+
+Hypothesis mergeBinds :
+  forall A B C (ga : G A) (gb : G B) (f : A -> B -> G C),
+    semGen (bindGen ga (fun x => bindGen gb (f x))) <-->
+    semGen (bindGen (genPair ga gb) (curry f)).
+
 End GenHighInterface.
 
 Module GenHigh : GenHighInterface.
